@prefix mv: <http://purl.org/net/mobivoc/> .
@prefix owl: <http://www.w3.org/2002/07/owl#> .
@prefix rdf: <http://www.w3.org/1999/02/22-rdf-syntax-ns#> .
@prefix rdfs: <http://www.w3.org/2000/01/rdf-schema#> .
@prefix skos: <http://www.w3.org/2004/02/skos/core#> .
#@prefix xsd

# CLASSES

mv:ParkingFacility
	a rdfs:Class , owl:Class ; 
	rdfs:comment "A parking lot or other parking facility with several parking spaces for vehicles." ;
	rdfs:label "parking facility"@en , "Parkeinrichtung"@de .

mv:ParkingFacilityFeature
	a rdfs:Class , owl:Class ;
	rdfs:comment "Features of the parking facility (e.g. parking for handicapped people)." ;
	rdfs:label "parking facility feature"@en , "Ausstattung der Parkeinrichtung"@de .

mv:ParkingFacilityService
	a rdfs:Class , owl:Class ;
	rdfs:comment "Service available at the parking facility." #at
	rdfs:label "services of parking facility"@en , "Serviceangebot der Parkeinrichtung"@de .

mv:ParkingLot
	a rdfs:Class, owl:Class ;
	rdfs:subClassOf mv:ParkingFacility ;
	rdfs:comment "Area used for parking vehicles with several parking spaces."
	skos:prefLabel "parking lot"@en-US , "car park"@en-UK , "Parkplatz"@de ;
	skos:hiddenLabel "car lot"@en , "Parkfläche"@de .

mv:ParkingGarage
	a rdfs:Class, owl:Class ;
	rdfs:subClassOf mv:ParkingFacility ;
	rdfs:comment "Building used for parking vehicles with one or several parking decks."
	skos:prefLabel "parking garage"@en , "Parkhaus"@de ;
	skos:hiddenLabel "multi-storey car park"@en , "parking structure"@en , "parking ramp"@en , "parkade"@en , 		"parking building"@en , "indoor parking"@en , "Hochgarage"@de .

mv:UndergroundParkingGarage
	a rdfs:Class, owl:Class ;
	rdfs:subClassOf mv:ParkingFacility ;
	rdfs:comment "Underground parking lot for parking vehicles with one or several parking decks."
	skos:prefLabel "underground parking garage"@en , "Tiefgarage"@de ;
	skos:hiddenLabel "Rampengarage"@de .


#INSTANCES

## Parking Facility Features

mv:ParkingSpaceForDisabledPerson #man könnte ja auch die Anzahl der Behindertenparkplätze angeben wollen, dann brauch ich doch ein Konzept?
	a mv:ParkingFacilityFeature ;
	rdfs:label "parking space for disabled persons"@en , "Behindertenparkplatz"@de.

mv:LadiesParkingSpace # wenn keine spezielleren Infos dran hängen, reicht eine property aus zb hasfrauenparkplätze und dann zahl.
	a mv:ParkingFacilityFeature ;
	rdfs:label "ladies' parking space" , "Frauenparkplatz"@de .

mv:XXLParkingSpace
	a mv:ParkingFacilityFeature ;
	rdfs:label "XXL parking space" , "XXL-Parkplatz"@de ;
	skos:altLabel "extra-breiter Stellplatz"@de .

mv:VideoSurveillance
	a mv:ParkingFacilityFeature ;
	rdfs:label "video surveillance"@en , "Videoüberwachung"@de .

mv:SurveillanceBySecurityGuards #check englische Bezeichnung
	a mv:ParkingFacilityFeature ;
	rdfs:label "surveillance by security guards"@en , "Bewacht durch Personal"@de ;
	skos:altLabel "personenbewacht"@de . #prüfen, ob das so hieß

mv:PayStation
	a mv:ParkingFacilityFeature ;
	rdfs:label "pay station"@en , "Kassenautomat"@de .

mv:ParkingBarrier
	a mv:ParkingFacilityFeature ;
	skos:preflabel "parking barrier"@en , "Parkschranke"@de.
	skos:altlabel "park barrier"@en

## Parking Facility Services

mv:ChargingPoint #welche konsequenzen hat hier die verwendung von charging point?-->als Property hasChargingPoints der ParkingFacility
	a mv:ParkingFacilityService
	# siehe ChargingPoint
	rdfs:label "charging point"@en , "Ladestation"@de .

mv:CarCleaningandMaintenance
	a mv:ParkingFacilityService ;
	rdfs:label "car cleaning and maintenance"@en , "Pkw-Reinigung und -Pflege"@de .


#PROPERTIES

mv:hasParkingFacilityFeatures
	a rdf:Property , owl:ObjectProperty ;
	rdfs:label "has parking facility feature" ;
	rdfs:comment "Indicates which features the parking facility provides."
	rdfs:domain mv:ParkingFacility ;
	rdfs:range mv:ParkingFacilityFeature .

mv:offersServices
	a rdf:Property , owl:ObjectProperty ;
	rdfs:label "offers services" ;
	rdfs:comment "Indicates which services are available at the parking facility." #at
	rdfs:domain mv:ParkingFacility ;
	rdfs:range mv:ParkingFacilityService .

mv:maximumNumberOfParkingSpaces
	a rdf:Property , owl:DatatypeProperty ;
	rdfs:label "maximum number of parking spaces" ;
	rdfs:comment "Indicates the maximum number of parking spaces of the parking facility." ;
	rdfs:domain mv:ParkingFacility ;
	rdfs:range xsd:integer .

mv:parkingSpacesOccupied
	a rdf:Property , owl:DatatypeProperty ;
	rdfs:label "parking spaces occupied" ;
	rdfs:comment "Indicates how many parking spaces of the parking facility are currently occupied." ;
	rdfs:domain mv:ParkingFacility ;
	rdfs:range xsd:integer .
	
mv:parkingSpacesVacant
	a rdf:Property , owl:DatatypeProperty ;
	rdfs:label "parking spaces vacant" ;
	rdfs:comment "Indicates how many parking spaces of the parking facility are currently vacant." ;
	rdfs:domain mv:ParkingFacility ;
	rdfs:range xsd:integer .
